\newcommand{\CLexcludedMiddle}{A \vee \neg A}
\newcommand{\CLaxiom}[1]{\AxiomC {$#1 \fCenter #1$}}
\newcommand{\CLconj}{\wedge}
\newcommand{\CLdisj}{\vee}
\newcommand{\CLimp}{\to}

\def\fCenter{\LLvdash}

\newcommand{\CLnegRule}{
\begin{center}
\begin{prooftree}
\RightLabel{L$\neg$}
\AxiomC {$\Gamma \fCenter A,\Delta$}
\UnaryInfC  {$\Gamma,\neg{A} \fCenter \Delta$}
	\DisplayProof \hskip 96pt
\RightLabel{R$\neg$}
\AxiomC {$\Gamma,A \fCenter \Delta$}
\UnaryInfC  {$\Gamma \fCenter \neg{A},\Delta$}
\end{prooftree}
\end{center}
}

\begin{table}
\begin{center}
\begin{prooftree}
\RightLabel{Ax}\AxiomC{} \UnaryInfC {$A \fCenter A$}
	\DisplayProof \hskip 48pt
\RightLabel{Cut}
\AxiomC {$\Gamma_0 \fCenter A,\Delta_0$}
\AxiomC {$\Gamma_1,A \fCenter \Delta_1$}
\BinaryInfC  {$\Gamma_0,\Gamma_1 \fCenter \Delta_0,\Delta_1$}
\end{prooftree}
\end{center}
%%

\begin{center}
\begin{prooftree}
\AxiomC {$\Gamma,A,A\fCenter\Delta$} \RightLabel{LC} \UnaryInfC {$\Gamma,A\fCenter\Delta$}
	\DisplayProof \hskip 18pt
\AxiomC {$\Gamma\fCenter A,A,\Delta$}
\RightLabel{RC} \UnaryInfC {$\Gamma\fCenter A,\Delta$}
	\DisplayProof \hskip 18pt\AxiomC {$\Gamma\fCenter\Delta$} \RightLabel{LW} \UnaryInfC {$\Gamma,A\fCenter\Delta$}
	\DisplayProof \hskip 18pt
\AxiomC {$\Gamma\fCenter\Delta$} 
\RightLabel{RW} \UnaryInfC {$\Gamma\fCenter A,\Delta$}
\end{prooftree}
\end{center}
%%
\begin{center}
\begin{prooftree}
\AxiomC {$\Gamma\fCenter\Delta$} \RightLabel{L$\top$} 
\UnaryInfC {$\Gamma,\top\fCenter\Delta$}
	\DisplayProof \hskip 18pt
\RightLabel{R$\top$} \AxiomC{} \UnaryInfC {$\Gamma\fCenter \top,\Delta$}
	\DisplayProof \hskip 18pt
\RightLabel{L$\bot$} \AxiomC{}\UnaryInfC {$\Gamma,\bot\fCenter\Delta$} 
	\DisplayProof \hskip 18pt
\AxiomC {$\Gamma\fCenter\Delta$} \RightLabel{R$\bot$} 
\UnaryInfC {$\Gamma\fCenter \bot,\Delta$}
\end{prooftree}
\end{center}
%%
\CLnegRule
%%
\begin{center}
\begin{prooftree}
\RightLabel{L$\CLimp$}
\AxiomC {$\Gamma_0 \fCenter A,\Delta_0$}
\AxiomC {$\Gamma_1,B \fCenter \Delta_1$}
\BinaryInfC  {$\Gamma_0,\Gamma_1,A\CLimp B \fCenter \Delta_0,\Delta_1$}
%
\DisplayProof \hskip 48pt
%
\RightLabel{R$\CLimp$}
\AxiomC {$\Gamma,A \fCenter B,\Delta$}
\UnaryInfC  {$\Gamma \fCenter A\CLimp B,\Delta$}
\end{prooftree}
\end{center}
%%
%%
\begin{center}
\begin{prooftree}
\RightLabel{L$\CLconj$ $(i = 1,2)$}
\AxiomC {$\Gamma,A_i \fCenter \Delta$}
\UnaryInfC  {$\Gamma,A_1 \CLconj A_2 \fCenter \Delta$}
%
\DisplayProof \hskip 64pt
%
\RightLabel{R$\CLconj$}
\AxiomC {$\Gamma \fCenter A,\Delta$}
\AxiomC {$\Gamma \fCenter B,\Delta$}
\BinaryInfC  {$\Gamma \fCenter A\CLconj B,\Delta$}
\end{prooftree}
\end{center}
%%
\begin{center}
\begin{prooftree}
\RightLabel{L$\CLdisj$}
\AxiomC {$\Gamma,A \fCenter \Delta$}
\AxiomC {$\Gamma,B \fCenter \Delta$}
\BinaryInfC  {$\Gamma,A\CLdisj B, \fCenter \Delta$}
%
\DisplayProof
\hskip 64pt
%
\RightLabel{R$\CLdisj$ $(i = 1,2)$}
\AxiomC {$\Gamma \fCenter A_i,\Delta$}
\UnaryInfC  {$\Gamma \fCenter A_1 \CLdisj A_2,\Delta$}
%
\end{prooftree}
\end{center}
%%
\caption{Classical Logic}
\end{table}

\begin{table}
\begin{center}
\begin{prooftree}
\CLaxiom{A}  
\RightLabel{Weakening} \UnaryInfC  {$A \fCenter B,A$}
\UnaryInfC  {$ \fCenter A \to B,A$}
\CLaxiom{A}
\BinaryInfC{$ (A \to B) \to A \fCenter A,A$}
\RightLabel{Contraction}  \UnaryInfC{$ (A \to B) \to A \fCenter A$}
\UnaryInfC{$  \fCenter ((A \to B) \to A) \to A$}
%
\DisplayProof
\hskip 48pt
%
\CLaxiom{A}
\UnaryInfC  {$A \fCenter \CLexcludedMiddle$}
\UnaryInfC  { $\fCenter \neg A,\CLexcludedMiddle$}
\UnaryInfC  {$ \fCenter \CLexcludedMiddle, \CLexcludedMiddle$}
\UnaryInfC  {$ \fCenter \CLexcludedMiddle$}
\end{prooftree}
\end{center}
\caption{pierce's law  and excluded middle}
\end{table}

\begin{table}
\begin{center}\begin{prooftree}
\AxiomC{[$A$] \scriptsize{1}} \AxiomC{[$\neg A$] \scriptsize{2}}
\BinaryInfC {$\bot$}
\UnaryInfC{$B$}
\RightLabel{$\to$ (1)} \UnaryInfC {$A \to B$}
\AxiomC {[$(A \to B) \to A$] \scriptsize{3}}
\BinaryInfC {$A$}
\AxiomC{[$\neg A$] \scriptsize{2}}
\BinaryInfC{$\bot$}
\RightLabel{$\to$ (2)} \UnaryInfC{$\neg\neg A$}
\UnaryInfC{$A$}
\RightLabel{$\to$ (3)} \UnaryInfC {$((A \to B) \to A) \to A$}
\end{prooftree}\end{center}
\caption{pierce's law in natural deduction style}
\end{table}

